\documentclass[12pt, a4paper]{IEEEtran}
    \usepackage{amsmath}
    \usepackage[pdftex]{graphicx}
    \usepackage{float}
    %设置四周
    \usepackage[left=1in, right=1in]{geometry}
    %设置字体
    \usepackage{times}
    \usepackage{mathptmx}
    %设置行距
    \linespread{0.3}
    %开始
    
    \begin{document}
    \centerline{\textbf{Name: Chen Chen}}
    \centerline{\textbf{UID: 004710308}}
    \centerline{\textbf{Dis 2A}}

    \section*{section 2.1}
    \subsection*{1}
    $$\o (t, y, y')=t^2y'+(1+t)y=0$$
    $$y'=-\frac{(1+t)y}{t^2}$$

    \subsection*{8}
    \subsection*{(a)}
    $$(t^2+y^2)'=(C^2)'$$
    $$\Rightarrow 2t+2yy'=0$$
    $$\Rightarrow t+yy'=0$$

    \subsection*{(b)}
    $$y=\pm \sqrt{C^2 -t^2}$$
    $$\Rightarrow y'=\mp \frac{t}{\sqrt{C^2-t^2}}$$
    plug into $t+yy'=0:$
    $$t+\frac{\pm \sqrt{C^2 -t^2}t}{\mp \sqrt{C^2-t^2}}=0$$
    $$\Rightarrow t-t=0$$

    \subsection*{(c)}
    $$Because , \sqrt{C^2-t^2}\geq 0$$
    $$\Rightarrow C^2 \geq t^2$$
    $$\Rightarrow -C\leq t \leq C$$

    \subsection*{(d)}
    \vspace{6cm}
    \subsection*{15}
    \vspace{6cm}
    \subsection*{20}
    \vspace{6cm}

    \section*{section 2.2}
    \subsection*{9}
    $$\frac{dy}{dx}=\frac{yIny}{x+1}$$
    $$\int \frac{dy}{yIny}=\int \frac{dx}{x+1}$$
    $$In|In(y)|=In|x+1|$$
    $$In(y)=x+1$$
    $$y=e^{x+1}$$

    \subsection*{15}
    $$\int ydy =\int sinx dx$$
    $$\frac{1}{2}y^2+C=-cosx+C$$
    $$y(x)=\pm\sqrt{-2cosx+C}$$
    plug in x=$\frac{\pi}{2}$
    $$y(x)=\sqrt{-2cosx+1}$$
    Interval of existence:
    $$-2cosx+1 \geq 0$$
    $$\Rightarrow \frac{\pi}{3}\textless x\textless\frac{5\pi}{3} $$


    \subsection*{22}
    $$\int \frac{y}{y^2+1}dy=\int dx$$
    $$In|y^2+1|+C=x+C$$
    $$y^2+1=e^{2x+2C}$$
    Because $e^{2C}$ is a constant, we can substitute it with $u$.
    $$y(x)=\pm \sqrt{ue^{2x}-1}$$
    plug in $x=1$
    $$4=ue^2-1$$
    $$u=5e^{-2}$$
    So, solution is:
    $$y(x)=\sqrt{5e^{2x-2}-1}$$
    Interval of existence:
    $$5e^{2x-2}-1\textgreater 0$$
    $$x>1-\frac{In(5)}{2}$$

    \subsection*{24}
    \subsection*{a}
    $$\lambda =1.551*10^{-8} $$
    \subsection*{b}
    $$N_0=1000 and N(t)=100$$
    $$t=In \frac{10}{\lambda}=1.485\times10^8 years$$
    
    
    \section*{section 2.4}
    \subsection*{8}
    $$u(x)=e^{-In(1+x^3)}=\frac{1}{1+x^3}$$
    $$\frac{1}{1+x^3}y'-\frac{3x^2}{(1+x^3)^2}y=\frac{x^2}{1+x^3}$$
    $$y(x)=\frac{1}{3(1+x^3)In(1+x^3)}+C(1+x^3)$$


    \subsection*{13}
    \subsection*{a}
    $$u(x)=e^{-\int a(x)dx}=e^{sinx}$$
    $$e^{sinx}(y'+ycosx)=e^{sinx}cosx$$
    $$e^{sinx}y=e^{sinx}+C$$
    $$y(x)=\frac{e^{sinx}+C}{e^{sinx}}$$

    \subsection*{b}
    $$\frac{dy}{1-y}=cosx dx$$
    $$-In|1-y|=sinx+C$$
    $$|1-y|=e^{-sinx-C}\Rightarrow 1-y=\pm e^{-sinx-C}$$
    let u=$\pm e^{-C}$
    $$y(x)=1-ue^{-sinx}$$


    \subsection*{19}
    $$u(x)=e^{\int -\frac{1}{2x+3}dx}=|2x+3|^{-\frac{1}{2}}$$
    $$(2x+3)^{-\frac{1}{2}}y'-(2x+3)^{-\frac{3}{2}}=(2x+3)^{-1}$$
    $$y(x)=\frac{1}{2}(2x+3)^{\frac{1}{2}}In(2x+3)+C(2x+3)^{\frac{1}{2}}$$
    Because $y(-1)=0=C$,
    $$y(x)=\frac{1}{2}(2x+3)^{\frac{1}{2}}In(2x+3).$$
    interval of existence:
    ($-\frac{3}{2}$, $+\infty$)
    
    
    \vspace{6cm}
    \subsection*{24}
    let $z=y^{-1}$
    $$\frac{dz}{dx}=\frac{dz}{dy}\frac{dy}{dx}=y^{-2}(y^2-y)=-1+z$$
    $$e^{-x}(\frac{dz}{dx}-z)=-e^{-x}$$
    $$\Rightarrow e^{-x}z=e^{-x}+C$$
    $$\Rightarrow z(x)=1+Ce^{x}$$
plug in $z=y^{-1}$
$$y(x)=\frac{1}{1+Ce^x}$$

    \end{document}