\documentclass[12pt, a4paper]{IEEEtran}
    \usepackage{amsmath}
    \usepackage[pdftex]{graphicx}
    \usepackage{float}
    \usepackage{ tipa }
    \usepackage{ dsfont }
    %设置四周
    \usepackage[left=1in, right=1in]{geometry}
    %设置字体
    \usepackage{times}
    \usepackage{mathptmx}
    %设置行距
    \linespread{0.7}
    %开始
    
    \begin{document}
    \centerline{\textbf{Name: Chen Chen}}
    \centerline{\textbf{UID: 004710308}}
    \centerline{\textbf{Dis 2A}}

    \section*{4.4}
    
    \subsection*{8}
    \vspace{6cm}
    $$tan \o =-\frac{1}{\sqrt{3}}\Rightarrow \o=-\frac{\pi}{6}$$
    
    \subsection*{11}
    $$0.2y''+5y=0 or y''+25y=0$$
    $$\lambda^2+25=0\Rightarrow \lambda=\pm 5$$
    $$y(t)=C_1cos5t+C_2sin5t$$
    $$\Rightarrow y'(t)=-5C_1sin5t+5C_2cos5t$$
    $$y(0)=0.5\Rightarrow C_1=0.5, y'(0)=0\Rightarrow C_2=0$$
    $$y(t)=0.5cos5t$$
    \vspace{6cm}

    \subsection*{16}
    \subsubsection*{a}
    $$k=2kg/s^2$$
    \subsubsection*{b}
    $$y''+3y'+2y=0\Rightarrow w_0=\sqrt{2}, c=1.5$$
    $$\lambda^2+3\lambda+2=0\Rightarrow \lambda_1=-1 \lambda_2=-2$$
    $$y(t)=C_1e^{-t}+C_2^{-2t}\Rightarrow y'(t)=-C_1e^{-t}-2C_2e^{-2t}$$
    $$y(t)=-3e^{-t}+2e^{-2t}$$
    \vspace{6cm}

    \subsection*{22}
    $$k=1.5kg/s$$
    $0.1y''+1.5y'+9.8y=0$ or $y''+15y'+98y=0$
    $$\lambda^2+15\lambda+98=0\Rightarrow \lambda=\frac{-15\pm\sqrt{167}i}{2}$$
    $$y(t)=e^{-\frac{15t}{2}}(C_1cos\frac{167}{2}t+C_2sin\frac{167}{2}t)$$
    $$C_1=\frac{1}{10} C_2\approx 0.12$$
    $$A=\sqrt{C_1^2+C_2^2}=\approx 0.15, \o \approx 0.86$$
    \vspace{6cm}

    \section*{4.5}
    \subsection*{2}
    $$y(t)=ae^{-t}\Rightarrow y'(t)=-ae^{-t} \Rightarrow y''(t)=ae^{-t}$$
    $$(ae^{-t})+6(-ae^{-t})+8(ae^{-t})=-3e^{-t}$$
    $$a=3\Rightarrow y_{p}=3e^{-t}$$    

    \subsection*{8}
    $$y(t)=acos3t+bsin3t$$
    $$y'(t)=-3asin3t+3cos3t$$
    $$y''(t)=-9acos3t-9bsin3t$$
    $$-9acos3t-9bsin3t+7(-3asin3t+3cos3t)+$$
    $$6(y(t)=acos3t+bsin3t)=-4sin3t$$
    $\Rightarrow a+21b=0$ and $-21a+b=-4$
    $$a=\frac{42}{221}, b=-\frac{2}{221}$$
    $$y_{p}=\frac{42}{221}cos3t-\frac{2}{221}sin3t$$

    \subsection*{12}
    $$z=Ae^{i2t}$$
    $$((2i)^2+7(2i)+6)A=3\Rightarrow A=\frac{3}{100}-\frac{21i}{100}$$
    $$z=(\frac{3}{100}-\frac{21i}{100})(cos2t+isin2t)$$
    $$y(t)=-\frac{21}{100}cos2t+\frac{3}{100}sin2t$$

    \subsection*{16}
    $$y(t)=at^2+bt+c$$
    $$y'(t)=2at+b$$
    $$y''(t)=2a$$
    $$2a+5(2at+b)+6(at^2+bt+c)=-t^2+4$$
    $$a=-\frac{1}{6},b=\frac{5}{18},c=\frac{53}{108}$$
    $$y(t)=-\frac{1}{6}t^2+\frac{5}{18}t+\frac{53}{108}$$

    \subsection*{20}
    $$y_h=e^{-t}(C_1costt+C_2sint)$$
    $$z=Ae^{i2t}\Rightarrow z'=(2i)Ai2t \Rightarrow z''=4i^2Ae^{i2t}$$
    $$A=-\frac{1}{5}-\frac{2}{5}i$$
    $$y_p=\frac{1}{5}cos2t+\frac{2}{5}sin2t$$
    $$y(t)=e^{-t}(C_1costt+C_2sint)+\frac{1}{5}cos2t+\frac{2}{5}sin2t$$
    $$C_1=-\frac{9}{5} C_2=-\frac{13}{5}$$
    $$y(t)=e^{-t}(-\frac{9}{5}costt+-\frac{13}{5}sint)+\frac{1}{5}cos2t+\frac{2}{5}sin2t$$

    \subsection*{28}
    $$y_h=(C_1+C_2t)e^{-2t}$$
    $$y_p(t)=Ate^{=2t}$$
    $$y_p'(t)=2Ae^{-2t}(t-t^2)$$
    $$y+p''(t)=2Ae^{-2t}(2t^2-4t+1)$$
    $$A=1$$
    $$y_p=t^2e^{-2t}$$

    \subsection*{33}
    $$y=at+b$$
    $$25at+25b=2+3t$$
    $$y=\frac{2}{25}t+\frac{3}{25}$$
    $$\lambda^2+25=0\Rightarrow \lambda=\pm 5i$$
    $$z=Ate^{5it}$$
    $$A=-\frac{1}{10i}$$
    $$z=-\frac{1}{10}it(cos5t+isin5t)$$
    $$y=\frac{2}{25}t+\frac{3}{25}+\frac{1}{10}tsin5t$$

    \subsection*{40}
    $$y=(at+b)e^{-3t}$$
    $$y'=e^{-3t}((a-3b)-3at)$$
    $$y''=3e^{-3t}((-2a+3b)+3at)$$
    $$a=\frac{1}{20}, b=\frac{9}{400}$$
    $$y=(\frac{1}{20}t+\frac{9}{400})e^{-3t}$$
    \end{document}