\documentclass[12pt, a4paper]{IEEEtran}
    \usepackage{amsmath}
    \usepackage[pdftex]{graphicx}
    \usepackage{float}
    \usepackage{ tipa }
    \usepackage{ dsfont }
    %设置四周
    \usepackage[left=1in, right=1in]{geometry}
    %设置字体
    \usepackage{times}
    \usepackage{mathptmx}
    %设置行距
    \linespread{0.7}
    %开始
    
    \begin{document}
    \centerline{\textbf{Name: Chen Chen}}
    
    \centerline{\textbf{Dis 2A}}
\section *{section 2.5}
\subsection*{1}

\subsection*{a}
Let $y(t)$ is the amount of sugar in the tank.\\
$\frac{dy}{dt}$ is the rate of change of the sugar in the tank
$$\frac{dy}{dt}=0.6-3\frac{y}{100}$$
$$\Rightarrow y(t)=20(1-e^{\frac{3t}{100}})$$
$$y(20)=10(1-e^{-0.6})(lb)$$

\subsection*{b}
$$20(1-e^{\frac{3t}{100}})=15$$
$$t=\frac{100In4}{3}(mm)$$ 

\subsection*{c}
$$t\rightarrow \infty, y(t)\rightarrow 20$$

\subsection*{5}
Let $y(t)$ is the amount of salt in the tank.\\
$\frac{dy}{dt}$ is the rate of change of the salt in the tank
$$\frac{dy}{dt}=2-\frac{x}{10+t}$$
$$y(t)=10+t-\frac{100}{(10+t)}$$
$$y(15)=21(lb)$$

\subsection*{7}
\subsection*{a}
Let $y(t)$ is the amount of pollutant in the tank.\\
$\frac{dy}{dt}$ is the rate of change of the pollutant in the tank.
$$\frac{dy}{dt}=3-\frac{4x}{50+t}$$
$$y(t)=\frac{3}{5}t+30-\frac{187500000}{(50+t)^4}$$
\subsection*{b}
$$\frac{dy}{dt}=-\frac{2x}{30-t}$$
$$y(t)=\frac{215342}{9000000}(30-t)^2$$
$$t=8.7868(min)$$

\subsection*{14}
Let $y(t)$ is the amount of salt in the tank $\textsci$ \\
$\frac{dy}{dt}$ is the rate of change of the salt in the tank $\textsci$.
$$\frac{dy}{dt}=ab-\frac{b}{V}y$$
$$y(t)=aV+Ke^{-\frac{b}{V}t}$$
Because $y(0)=0$
$$K=-aV$$
Let $z(t)$ is the amount of salt in the tank $\mathds{I}$ \\
$\frac{dz}{dt}$ is the rate of change of the salt in the tank $\mathds{I}$.
$$\frac{dz}{dt}=\frac{b}{V}x-\frac{b}{V}y$$
$$y=aV-abte^{-\frac{b}{V}t}-aVe^{-\frac{b}{V}t}$$




\section*{section 2.6}
\subsection*{6}
$$\frac{\partial (In(xy)+x^2 y^3)}{\partial x}$$
$$\Rightarrow (\frac{1}{x}+2xy^3)dx$$
$$\frac{\partial (In(xy)+x^2 y^3)}{\partial y}$$
$$\Rightarrow (\frac{1}{y}+3x^2y^2)dy$$
$$dF=(\frac{1}{x}+2xy^3)dx+(\frac{1}{y}+3x^2y^2)dy$$
\subsection*{8}
$$\frac{\partial (tan^{-1}(\frac{x}{y})+y^4)}{\partial x}$$
$$\Rightarrow (\frac{y}{x^2+y^2})dx$$
$$\frac{\partial (tan^{-1}(\frac{x}{y})+y^4)}{\partial y}$$
$$\Rightarrow (-\frac{x}{x^2+y^2}+4y^3)dy$$
$$dF=(\frac{y}{x^2+y^2})dx+(-\frac{x}{x^2+y^2}+4y^3)dy$$

\subsection*{16}
$$\o(u,v)=\int \frac{2u}{u^2+v^2}du + g(v)$$
$$=In|v^2+u^2|+g(v)$$
$$\frac{\partial \o}{\partial v}=\frac{2v}{v^2+u^2}+g'(v)$$
$$\Rightarrow g'(v)=0 \Rightarrow g(v)=C$$
$$\o (u,v)=In|v^2+u^2|+C$$

\subsection*{24}
$$\frac{(3y+y)(y+1)}{x^4}dx+\frac{-2(y+1)}{x^3}dy$$

$$\o(x,y)=\int \frac{(3y+y)(y+1)}{x^4}dx +g(y)$$

$$=-\frac{4y(1+y)}{3x^3}+g(y)$$

$$\frac{\partial \o}{\partial y}=\frac{4+8y}{3x^3}+g'(y)=\frac{-2(y+1)}{x^3}$$
$$g'(y)=\int (-\frac{2(y+1)}{x^3}-\frac{4+8y}{3x^3})dy$$
$$g(y)=-\frac{2(\frac{7y^2}{2}+5y)}{3x^3}$$
$$\o(x,y)=-\frac{2(\frac{7y^2}{2}+5y)}{3x^3}-\frac{4y(1+y)}{3x^3}$$

\subsection*{29}
$$M=y^2+2xy, N=-x^2$$
$$\frac{\partial M}{\partial y}=2y+2x, \frac{\partial N}{\partial x}=-2x$$
$$\mu=e^{-\int \frac{2(2x+y)}{y(2x+y)}dx}$$
$$=e^{-2In y}=\frac{1}{y^2}$$
$$(1+\frac{2x}{y})dx-\frac{x^2}{y^2}dy=0$$
$$F(x,y)=\frac{xy+x^2}{y}=C$$
$$\mu (y)=\frac{1}{y^2}$$

\subsection*{38}
$$y=vx, \frac{dy}{dx}=v+\frac{dv}{dx}$$
$$\Rightarrow v+x\frac{dv}{dx}=\frac{v+v^3}{v^2-2}$$
$$x\frac{dv}{dx}=\frac{3v}{v^2-2}$$
$$\int (\frac{v^2-2}{3v})dv=\int \frac{dx}{x}$$
$$\Rightarrow \frac{v^2}{6}-\frac{2}{3}In(v)=In(x)+In(C)$$
$$y^{\frac{2}{3}}=Cx^{-\frac{1}{3}}e^{\frac{y^2}{6x^2}}$$
\end{document}