\documentclass[12pt, a4paper]{IEEEtran}
    \usepackage{amsmath}
    \usepackage[pdftex]{graphicx}
    \usepackage{float}
    \usepackage{ tipa }
    \usepackage{ dsfont }
    %设置四周
    \usepackage[left=1in, right=1in]{geometry}
    %设置字体
    \usepackage{times}
    \usepackage{mathptmx}
    %设置行距
    \linespread{0.7}
    %开始
    
    \begin{document}
    \centerline{\textbf{Name: Chen Chen}}
    \centerline{\textbf{UID: 004710308}}
    \centerline{\textbf{Dis 2A}}

    \section*{4.1}
    \subsection*{21}
    $$\left[
        \begin{matrix}
            t^2&t|t|\\
            2t&2|t|\\
        \end{matrix}
        \right]
    =2|t|t^2-2tt|t|=0$$
    So, it is linear dependent.

    \subsection*{22}
    
    $$\left[
        \begin{matrix}
            e^t&e^{-3t}\\
            e^t&-3e^{-3t}\\
        \end{matrix}
        \right]
    =-4e^{-2t}$$
    $$y(0)=1=C_1e^0+C_2e^{-3\times 0}=C_1+C_2=1$$
    $$y'(0)=-2=C_1e^0-C_23e^{-3\times 0}=C_1-(-3)C_2$$
    $$C_1=\frac{1}{4}, C_2=\frac{3}{4}$$

    \subsection*{27}
    $$y_2(t)=y_1(t)x=xt$$
    $$(xt)'=x't+x, (x't+x)'=x''t+2x'$$
    $$t^2(x''t+2x')-2t(x't+x)+2xt=0$$
    $$\Rightarrow t^3x''=0 \Rightarrow x''=0\Rightarrow x=t\Rightarrow y_2(t)=t^2$$
    $$t^2(2)-2t(2t)+2t^2=0$$
    $$y=C_1t+C_2t^2$$\\
    

    \section*{4.3}

    \subsection*{6}
    $$6\lambda^2+\lambda-1=0= (3\lambda-1)(2\lambda+1)$$
    $$\lambda_1=\frac{1}{3}, \lambda_2=-\frac{1}{2}$$
    $$y(t)=C_1e^{\frac{1}{3}}+C_2e^{-\frac{1}{2}}$$

    \subsection*{8}
    $$6\lambda+5\lambda-6=0=(2\lambda+3)(3\lambda-2)$$
    $$\lambda_1=\frac{2}{3}, \lambda_2=-\frac{3}{2}$$
    $$y(t)=C_1e^{\frac{2}{3}}+C_2e^{-\frac{3}{2}}$$

    \subsection*{14}
    $$\lambda^2+2\lambda+3=0$$
    $$\lambda=-1\pm \sqrt{2}i$$
    $$y(t)=e^{-t}(C_1cos\sqrt{2}t+C_2sin\sqrt{2}t)$$

    \subsection*{16}
    $$\lambda^2+2\lambda+2=0$$
    $$\lambda=-1\pm i$$
    $$y(t)=e^{-t}(C_1cost+C_2sint)$$

    \subsection*{20}
    $$4\lambda^2+12\lambda+0=9=(2\lambda+3)(2\lambda+3)$$
    $$\lambda=-\frac{3}{2}$$
    $$y(t)=C_1e^{-\frac{3}{2}t}-C_2te^{-\frac{3}{2}t}$$

    \subsection*{24}
    $$\lambda^2+8\lambda+16=(\lambda+4)(\lambda+4)=0$$
    $$\lambda=-4$$
    $$y(t)=C_1e^{-4t}+C_2te^{-4t}$$

    \subsection*{30}
    $$\lambda^2-2\lambda-3=(\lambda-3)(\lambda+1)=0$$
    $$\lambda_1=3, \lambda_2=-1$$
    $$y(t)=C_1e^{3t}+C_2e^{-t}$$

    \subsection*{38}
    Because $\lambda=\lambda_1$,\\
    $$\lambda^2+p\lambda+q=(\lambda-\lambda_1)(\lambda-\lambda_1)=\lambda^2-2\lambda_1\lambda+\lambda_1^2$$
    $$\Rightarrow p=-2\lambda_1, q=\lambda_1^2$$
    $$\frac{dy}{dt}=e^{\lambda_{1}t}+\lambda_1te^{\lambda_1t}$$
    $$\frac{d^2y}{dx^2}=\lambda_1e^{\lambda_1t}(2+\lambda_1t)$$
    plug in $\frac{dy}{dt}$ and $\frac{d^2y}{dx^2}$ into $y''+py'+qy$
    $$\Rightarrow \lambda_1e^{\lambda_1t}(2+\lambda_1t)+p(e^{\lambda_{1}t}+\lambda_1te^{\lambda_1t})-q(te^{\lambda_1t})$$
    plug in $p=-2\lambda_1$ and $ q=\lambda_1^2$
    $$\Rightarrow 2\lambda_1e^{\lambda_1t}+\lambda_1^2te^{\lambda_1t}-2\lambda_1e^{\lambda_1t}-2\lambda_1^2te^{\lambda_1t}+\lambda^2te^{\lambda_1t}=0$$
    

























    

    \end{document}