\documentclass[12pt, a4paper]{IEEEtran}
    \usepackage{amsmath}
    \usepackage[pdftex]{graphicx}
    \usepackage{float}
    \usepackage{ tipa }
    \usepackage{ dsfont }
    %设置四周
    \usepackage[left=1in, right=1in]{geometry}
    %设置字体
    \usepackage{times}
    \usepackage{mathptmx}
    %设置行距
    \linespread{1.2}
    %开始
    
    \begin{document}
    \centerline{\textbf{Name: Chen Chen}}
    \centerline{\textbf{UID: 004710308}}
    \centerline{\textbf{Dis 2A}}
    \begin{flushleft}
    \section*{4}
        $y(t)=Ae^{2t}$\\
        $y'(t)=2Ae^{2t}$\\
        $y''(t)=4Ae^{2t}$\\
        plug into $y''+3y'-18y=18e^{2t}$
        $4Ae^{2t}+6Ae^{2t}-18Ae^{2t}=18e^{2t}$\\
        $-8A=18\Rightarrow A=-\frac{9}{4}$\\
        $y(t)=-\frac{9}{4}e^{2t}$


    \section*{6}
    $y(t)=acos2t+bsin2t$\\
    $y'(t)=-2asin2t+2bcos2t$\\
    $y''(t)=-4acos2t-4bsin2t$\\
    plug into $y''+9y=sin2t$\\
    $-4acos2t-4bsin2t+9acost2t+9bsin2t=sin2t$\\
    \vspace{1ex}
    $\begin{cases}
    5b=1\\
    5a=0
    \end{cases}
    \Rightarrow
    \begin{cases}
        a=0\\
        b=\frac{1}{5}
    \end{cases}$\\
    $y(t)=\frac{1}{5}sin2t$


    \section*{14}
    $y(t)=At+B \Rightarrow y'(t)=A \Rightarrow y''(t)=0$\\
    plug into $y''+5y'+4y=2+3t$\\
    $4At+5A+4B=3t+2$\\
    \vspace{1ex}
    $\begin{cases}
        4A=3\\
        5A+4B=2
    \end{cases}
    \Rightarrow
    \begin{cases}
        A=\frac{3}{4}\\
        B=-\frac{7}{16}
    \end{cases}$\
    $y(t)=\frac{3}{4}t-\frac{7}{16}$

    \section*{18}
    $\lambda^2+3\lambda+2=0\Rightarrow (\lambda+1)(\lambda+2)=0$\\
    $\lambda_1=-1, \lambda_2=-2$\\
    $y_g(t)=C_1e^{-t}+C_2e^{-2t}$\\
    $y_p(t)=Ae^{-4t}$\\
    $y_p'(t)=-4Ae^{-4t}$\\
    $y_p''(t)=16Ae^{-4t}$\\
    plug into $y''+3y'+2y=3e^{-4t}$\\
    $16Ae^{-4t}-12Ae^{-4t}+2Ae^{-4t}=3e^{-4t}$\\
    $6A=3 \Rightarrow A=\frac{1}{2}$\\
    $y(t)=C_1e^{-t}+C_2e^{-2t}+\frac{1}{2}e^{-4t}$\\
    $y'(t)=-C_1e^{-t}-2C_2e^{-2t}-2e^{-4t}$\\
    Because $y(0)=1$ and $y'(0)=0$,\\
    $C_1=3, C_2=-\frac{5}{2}$\\
    $y(t)=3e^{-t}-\frac{5}{2}e^{-2t}+\frac{1}{2}e^{-4t}$\\

    \section*{22}
    $\lambda^2+4\lambda+4=0\Rightarrow(\lambda+2)^2=0$\\
    $\lambda=-2$\\
    $y_g(t)=C_1e^{-2t}+C_2te^{-2t}$\\
    $y_p(t)=At+B\Rightarrow y_p'(t)=A \Rightarrow y_p''(t)=0$\\
    plug into $y''+4y'+4y=4-t$\\
    $4A+4(At+B)=4-t$\\
    \vspace{1ex}
    $\begin{cases}
        4A=-1\\
        4B=5
    \end{cases}
    \Rightarrow
    \begin{cases}
        A=-\frac{1}{4}\\
        B=\frac{5}{4}
    \end{cases}$
    $y(t)=C_1e^{-2t}+C_2te^{-2t}-\frac{1}{4}t+\frac{5}{4}$\\
    $y'(t)=-2C_1e^{-2t}+C_2e^{-2t}-2C_2te^{-2t}-\frac{1}{4}$\\
    Because $y(0)=-1$ and $y'(0)=0$\\
    $C_1=-\frac{9}{4}, C_2=\frac{17}{4}$\\
    $y(t)=-\frac{9}{4}e^{-2t}+\frac{17}{4}te^{-2t}-\frac{1}{4}t+\frac{5}{4}$\\
    
    \section*{26}
    $y(t)=R\left\{4e^{2it}\right\}=R\left\{4(cos2t+isin2t)\right\}$\\
    $y_p(t)=Ate^{2it}$\\
    $y_p'(t)=At^{2it}+2itAe^{2it}$\\
    $y_p''(t)=4iAe^{2it}-4tAe^{2it}$\\
    $4iAe^{2it}-4tAe^{2it}+4Ate^{2it}=4e^{2it}$\\
    $A=-i$\\
    $z(t)=-it(cos2t+isin2t)=-itcos2t+sin2t$\\
    $R\left\{z(t)\right\}=y_p(t)=tsin2t$

    \section*{30}
    $\alpha y_f''+\alpha py_f'+\alpha qy_f=\alpha f(t)$\\
    $\beta y_g''+\beta y_g'+\beta y_g=\beta g(t)$\\
    $(\alpha y_f+\beta y_g)''+p(\alpha py_f+\beta y_g)'+q(\alpha py_f+\beta y_g)=\alpha f(t)+\beta g(t)$\\
    $\Rightarrow z(t)=\alpha f(t)+\beta g(t)$

    \section*{34}
    $y_1''+2y_1'+y_1=3$\\
    $y_2''+2y_2'+y_2=-e^{-t}$\\
    $y_{1p}=A,y_{1p}'=0,y_{1p}'=0$\\
    $A=3\Rightarrow y_{1p}=3$\\
    $y_{2p}=Ate^{-t}$\\
    $y_{2p}'=(A-At)e^{-t}$\\
    $y_{2p}''=(At-A)e^{-t}$\\
    $(At-A)e^{-t}+(2A-2At)e^{-t}+Ate^{-t}=-e^{-t}$\\
    $A=-1\Rightarrow y_{2p}=-e^{-t}$\\
    $y(t)=3-e^{-t}$\\
    
    \section*{36}
    $y_1''+2y_1'+2y_1=3cost$\\
    $y_2''+2y_2'+2y_2=-sint$\\
    $z(t)=Ae^{it},z'(t)=Aie^{it},z''(t)=i^2Ae^{it}$\\
    plug into $z''+2z'+2z=e^{it}$\\
    $A(i^2+2i+2)e^{it}=e^{it}$\\
    $A=\frac{1-2i}{5}\Rightarrow z(t)=\frac{1-2i}{5}(cost+isint)$\\
    $\frac{y_{1p}}{3}=R\left\{z(t)\right\}\frac{1}{5}cost+\frac{2}{5}sint$\\
    $y_{2p}=im\left\{z(t)\right\}=\frac{1}{5}sint-\frac{2}{5}cost$
    $y(t)=cost+sint$

    \section*{41}
    $y_p(t)=(At^2+Bt+C)e^{-2t}$\\
    $y_p'(t)=(-2At^2+2At-2Bt+B-2C)e^{-2t}$\\
    $y_p''(t)=(4At^2-8At+4Bt+2A-4B-4C)e^{-2t}$\\
    plug into $y''+2y'+y=t^2e^{-2t}$\\
    $\left\{(4At^2-8At+4Bt+2A-4B-4C)+\right .$\\
    $(-2At^2+2At-2Bt+B-2C)+$\\
    $\left .(At^2+Bt+C)\right\}e^{-2t}=t^2e^{-2t}$\\
    $At^2-4At+Bt+2A-2B+C=t^2$\\
    $\begin{cases}
        A=1\\
        -4A+B=0\\
        2A-2B+C=0
    \end{cases}
    \Rightarrow
    \begin{cases}
        A=1\\
        B=4\\
        C=6
    \end{cases}$\\
    $y(t)=(t^2+4t+6)e^{-2t}$

\section*{44}
$y_p(t)=(bsint+acost)e^{-2t}$\\
$y_p'(t)=\left\{(-a-2b)sint+(-2a+b)cost\right\}e^{-2t}$\\
$y_p''(t)=\left\{(4a+3b)sint+(3a-4b)cost\right\}e^{-2t}$\\
plug into $y''+2y'+2y=e^{-2t}sint$\\
$\left\{(4a+3b)sint+(3a-4b)cost\right .+$\\
$((-2a-4b)sint+(-4a+2b)cost)$+\\
$\left . (2bsint+2acost)\right\}e^{-2t}=e^{-2t}sint$\\
$\Rightarrow (2a+b)sint+(a-2b)cost=sint$\\
$\begin{cases}
    2a+b=1\\
    a-2b=0
\end{cases}
\Rightarrow
\begin{cases}
    a=\frac{2}{5}\\
    b=\frac{1}{5}
\end{cases}$\\
$y(t)=\frac{2}{5}cost+\frac{1}{5}sint$


    
        
    

\end{flushleft}
\end{document}